src/floating-point/fp-functor.sml
@@ -27,8 +27,12 @@ struct
 
    val (fp_abs_tm, mk_fp_abs, dest_fp_abs, is_fp_abs) = monop "abs"
    val (fp_add_tm, mk_fp_add, dest_fp_add, is_fp_add) = triop "add"
+   val (fp_add_with_flags_tm, mk_fp_add_with_flags, dest_fp_add_with_flags,
+        is_fp_add_with_flags) = triop "add_with_flags"
    val fp_bottom_tm = const "bottom"
    val (fp_div_tm, mk_fp_div, dest_fp_div, is_fp_div) = triop "div"
+   val (fp_div_with_flags_tm, mk_fp_div_with_flags, dest_fp_div_with_flags,
+        is_fp_div_with_flags) = triop "div_with_flags"
    val (fp_compare_tm, mk_fp_compare, dest_fp_compare, is_fp_compare) =
       binop "compare"
    val (fp_equal_tm, mk_fp_equal, dest_fp_equal, is_fp_equal) = binop "equal"
@@ -56,10 +60,18 @@ struct
    val (fp_lessThan_tm, mk_fp_lessThan, dest_fp_lessThan, is_fp_lessThan) =
       binop "lessThan"
    val (fp_mul_tm, mk_fp_mul, dest_fp_mul, is_fp_mul) = triop "mul"
+   val (fp_mul_with_flags_tm, mk_fp_mul_with_flags, dest_fp_mul_with_flags,
+        is_fp_mul_with_flags) = triop "mul_with_flags"
    val (fp_mul_add_tm, mk_fp_mul_add, dest_fp_mul_add, is_fp_mul_add) =
       quadop "mul_add"
+   val (fp_mul_add_with_flags_tm, mk_fp_mul_add_with_flags,
+        dest_fp_mul_add_with_flags, is_fp_mul_add_with_flags) =
+      quadop "mul_add_with_flags"
    val (fp_mul_sub_tm, mk_fp_mul_sub, dest_fp_mul_sub, is_fp_mul_sub) =
       quadop "mul_sub"
+   val (fp_mul_sub_with_flags_tm, mk_fp_mul_sub_with_flags,
+        dest_fp_mul_sub_with_flags, is_fp_mul_sub_with_flags) =
+      quadop "mul_sub_with_flags"
    val fp_neginf_tm = const "negInf"
    val fp_negmin_tm = const "negMin"
    val fp_negzero_tm = const "negZero"
@@ -71,7 +83,11 @@ struct
    val (fp_roundToIntegral_tm, mk_fp_roundToIntegral, dest_fp_roundToIntegral,
         is_fp_roundToIntegral) = binop "roundToIntegral"
    val (fp_sqrt_tm, mk_fp_sqrt, dest_fp_sqrt, is_fp_sqrt) = binop "sqrt"
+   val (fp_sqrt_with_flags_tm, mk_fp_sqrt_with_flags, dest_fp_sqrt_with_flags,
+        is_fp_sqrt_with_flags) = binop "sqrt_with_flags"
    val (fp_sub_tm, mk_fp_sub, dest_fp_sub, is_fp_sub) = triop "sub"
+   val (fp_sub_with_flags_tm, mk_fp_sub_with_flags, dest_fp_sub_with_flags,
+        is_fp_sub_with_flags) = triop "sub_with_flags"
    val (fp_to_float_tm, mk_fp_to_float, dest_fp_to_float, is_fp_to_float) =
       monop "to_float"
    val (fp_to_int_tm, mk_fp_to_int, dest_fp_to_int, is_fp_to_int) =
