src/floating-point/fp-sig.sml
@@ -5,9 +5,11 @@ sig
     val float_to_fp_tm : term
     val fp_abs_tm : term
     val fp_add_tm : term
+    val fp_add_with_flags_tm : term
     val fp_bottom_tm : term
     val fp_compare_tm : term
     val fp_div_tm : term
+    val fp_div_with_flags_tm : term
     val fp_equal_tm : term
     val fp_greaterEqual_tm : term
     val fp_greaterThan_tm : term
@@ -22,8 +24,11 @@ sig
     val fp_lessEqual_tm : term
     val fp_lessThan_tm : term
     val fp_mul_tm : term
+    val fp_mul_with_flags_tm : term
     val fp_mul_add_tm : term
+    val fp_mul_add_with_flags_tm : term
     val fp_mul_sub_tm : term
+    val fp_mul_sub_with_flags_tm : term
     val fp_negate_tm : term
     val fp_neginf_tm : term
     val fp_negmin_tm : term
@@ -33,7 +38,9 @@ sig
     val fp_poszero_tm : term
     val fp_roundToIntegral_tm : term
     val fp_sqrt_tm : term
+    val fp_sqrt_with_flags_tm : term
     val fp_sub_tm : term
+    val fp_sub_with_flags_tm : term
     val fp_to_float_tm : term
     val fp_to_int_tm : term
     val fp_to_real_tm : term
@@ -44,8 +51,10 @@ sig
     val mk_float_to_fp : term -> term
     val mk_fp_abs : term -> term
     val mk_fp_add : term * term * term -> term
+    val mk_fp_add_with_flags : term * term * term -> term
     val mk_fp_compare : term * term -> term
     val mk_fp_div : term * term * term -> term
+    val mk_fp_div_with_flags : term * term * term -> term
     val mk_fp_equal : term * term -> term
     val mk_fp_greaterEqual : term * term -> term
     val mk_fp_greaterThan : term * term -> term
@@ -60,12 +69,17 @@ sig
     val mk_fp_lessEqual : term * term -> term
     val mk_fp_lessThan : term * term -> term
     val mk_fp_mul : term * term * term -> term
+    val mk_fp_mul_with_flags : term * term * term -> term
     val mk_fp_mul_add : term * term * term * term -> term
+    val mk_fp_mul_add_with_flags : term * term * term * term -> term
     val mk_fp_mul_sub : term * term * term * term -> term
+    val mk_fp_mul_sub_with_flags : term * term * term * term -> term
     val mk_fp_negate : term -> term
     val mk_fp_roundToIntegral : term * term -> term
     val mk_fp_sqrt : term * term -> term
+    val mk_fp_sqrt_with_flags : term * term -> term
     val mk_fp_sub : term * term * term -> term
+    val mk_fp_sub_with_flags : term * term * term -> term
     val mk_fp_to_float : term -> term
     val mk_fp_to_int : term * term -> term
     val mk_fp_to_real : term -> term
@@ -75,8 +89,10 @@ sig
     val is_float_to_fp : term -> bool
     val is_fp_abs : term -> bool
     val is_fp_add : term -> bool
+    val is_fp_add_with_flags : term -> bool
     val is_fp_compare : term -> bool
     val is_fp_div : term -> bool
+    val is_fp_div_with_flags : term -> bool
     val is_fp_equal : term -> bool
     val is_fp_greaterEqual : term -> bool
     val is_fp_greaterThan : term -> bool
@@ -90,12 +106,17 @@ sig
     val is_fp_lessEqual : term -> bool
     val is_fp_lessThan : term -> bool
     val is_fp_mul : term -> bool
+    val is_fp_mul_with_flags : term -> bool
     val is_fp_mul_add : term -> bool
+    val is_fp_mul_add_with_flags : term -> bool
     val is_fp_mul_sub : term -> bool
+    val is_fp_mul_sub_with_flags : term -> bool
     val is_fp_negate : term -> bool
     val is_fp_roundToIntegral : term -> bool
     val is_fp_sqrt : term -> bool
+    val is_fp_sqrt_with_flags : term -> bool
     val is_fp_sub : term -> bool
+    val is_fp_sub_with_flags : term -> bool
     val is_fp_to_float : term -> bool
     val is_fp_to_int : term -> bool
     val is_fp_to_real : term -> bool
@@ -105,8 +126,10 @@ sig
     val dest_float_to_fp : term -> term
     val dest_fp_abs : term -> term
     val dest_fp_add : term -> term * term * term
+    val dest_fp_add_with_flags : term -> term * term * term
     val dest_fp_compare : term -> term * term
     val dest_fp_div : term -> term * term * term
+    val dest_fp_div_with_flags : term -> term * term * term
     val dest_fp_equal : term -> term * term
     val dest_fp_greaterEqual : term -> term * term
     val dest_fp_greaterThan : term -> term * term
@@ -121,12 +144,17 @@ sig
     val dest_fp_lessEqual : term -> term * term
     val dest_fp_lessThan : term -> term * term
     val dest_fp_mul : term -> term * term * term
+    val dest_fp_mul_with_flags : term -> term * term * term
     val dest_fp_mul_add : term -> term * term * term * term
+    val dest_fp_mul_add_with_flags : term -> term * term * term * term
     val dest_fp_mul_sub : term -> term * term * term * term
+    val dest_fp_mul_sub_with_flags : term -> term * term * term * term
     val dest_fp_negate : term -> term
     val dest_fp_roundToIntegral : term -> term * term
     val dest_fp_sqrt : term -> term * term
+    val dest_fp_sqrt_with_flags : term -> term * term
     val dest_fp_sub : term -> term * term * term
+    val dest_fp_sub_with_flags : term -> term * term * term
     val dest_fp_to_float : term -> term
     val dest_fp_to_int : term -> term * term
     val dest_fp_to_real : term -> term
